backend/Inliningproof_linker.v
@@ -1,0 +1,1013 @@
+Require Import Coqlib.
+Require Import Errors.
+Require Import Maps.
+Require Import AST.
+Require Import Integers.
+Require Import Values.
+Require Import Memory.
+Require Import Globalenvs.
+Require Import Events.
+Require Import Smallstep.
+Require Import Op.
+Require Import Registers.
+Require Import Inlining.
+Require Import Inliningspec.
+Require Import RTL.
+Require Import Inliningproof.
+Require Import LinkerSpecification.
+Require Import Linkeq ProgramSim.
+Require Import RTLSim MemoryRelation.
+Require Import WFType paco.
+
+Set Implicit Arguments.
+
+Section INLINING.
+
+Let transf_EF (ef:external_function) := OK ef.
+Let transf_V (v_src:unit) := OK v_src.
+Let fundef_dec := (@common_fundef_dec function).
+
+Variable prog: program.
+Variable tprog: program.
+Hypothesis TRANSF: transf_program prog = OK tprog.
+
+Let fenv := funenv_program prog.
+
+Section FUTURE.
+
+Variable (fprog ftprog:program).
+Hypothesis (Hfsim:
+              program_weak_sim
+                fundef_dec fn_sig fundef_dec fn_sig transf_V
+                fprog ftprog).
+
+Hypothesis (Hfprog: program_linkeq (@common_fundef_dec function) prog fprog).
+Hypothesis (Hftprog: program_linkeq (@common_fundef_dec function) tprog ftprog).
+
+Let globfun_weak_sim :=
+  globfun_sim fundef_dec fn_sig fundef_dec fn_sig (fun _ _ _ _ => True) fprog ftprog.
+
+Let ge := Genv.globalenv fprog.
+Let tge := Genv.globalenv ftprog.
+
+(* TODO: duplicated lemmas of CSEproof_linker. Modularize? *)
+
+Lemma symbols_preserved:
+  forall (s: ident), Genv.find_symbol tge s = Genv.find_symbol ge s.
+Proof (symbols_preserved Hfsim).
+
+Lemma varinfo_preserved:
+  forall b, Genv.find_var_info tge b = Genv.find_var_info ge b.
+Proof.
+  intros. exploit varinfo_preserved.
+  { instantiate (1 := ftprog). instantiate (1 := fprog). apply Hfsim. }
+  instantiate (1 := b). unfold ge, tge.
+  destruct (Genv.find_var_info (Genv.globalenv ftprog) b), (Genv.find_var_info (Genv.globalenv fprog) b); intros; auto; inv H.
+  destruct g0; auto.
+Qed.
+
+Lemma funct_ptr_translated:
+  forall (b: block) (f: RTL.fundef),
+  Genv.find_funct_ptr ge b = Some f ->
+  exists tf, Genv.find_funct_ptr tge b = Some tf /\
+             fundef_weak_sim
+               (@common_fundef_dec function) fn_sig
+               (@common_fundef_dec function) fn_sig
+               ge tge f tf.
+Proof (funct_ptr_translated Hfsim).
+
+Lemma functions_translated:
+  forall (v: val) (f: RTL.fundef),
+  Genv.find_funct ge v = Some f ->
+  exists tf, Genv.find_funct tge v = Some tf /\
+             fundef_weak_sim
+               (@common_fundef_dec function) fn_sig
+               (@common_fundef_dec function) fn_sig
+               ge tge f tf.
+Proof (functions_translated Hfsim).
+
+Lemma sig_preserved:
+  forall f tf,
+    fundef_weak_sim
+      (@common_fundef_dec function) fn_sig
+      (@common_fundef_dec function) fn_sig
+      ge tge f tf ->
+    funsig tf = funsig f.
+Proof.
+  intros. inv H. inv Hsig. unfold common_fundef_dec in *.
+  destruct f, tf; simpl in *; auto.
+Qed.
+
+(** ** Relating global environments *)
+
+Inductive match_globalenvs (F: meminj) (bound: block): Prop :=
+  | mk_match_globalenvs
+      (DOMAIN: forall b, Plt b bound -> F b = Some(b, 0))
+      (IMAGE: forall b1 b2 delta, F b1 = Some(b2, delta) -> Plt b2 bound -> b1 = b2)
+      (SYMBOLS: forall id b, Genv.find_symbol ge id = Some b -> Plt b bound)
+      (FUNCTIONS: forall b fd, Genv.find_funct_ptr ge b = Some fd -> Plt b bound)
+      (VARINFOS: forall b gv, Genv.find_var_info ge b = Some gv -> Plt b bound).
+
+Lemma find_function_agree:
+  forall ros rs fd F ctx rs' bound,
+  find_function ge ros rs = Some fd ->
+  agree_regs F ctx rs rs' ->
+  match_globalenvs F bound ->
+  exists fd',
+  find_function tge (sros ctx ros) rs' = Some fd' /\
+  fundef_weak_sim
+    (@common_fundef_dec function) fn_sig
+    (@common_fundef_dec function) fn_sig
+    ge tge fd fd'.
+Proof.
+  intros. destruct ros as [r | id]; simpl in *.
+  (* register *)
+  assert (rs'#(sreg ctx r) = rs#r).
+    exploit Genv.find_funct_inv; eauto. intros [b EQ].
+    assert (A: val_inject F rs#r rs'#(sreg ctx r)). eapply agree_val_reg; eauto.
+    rewrite EQ in A; inv A.
+    inv H1. rewrite DOMAIN in H5. inv H5. auto.
+    apply FUNCTIONS with fd. 
+    rewrite EQ in H; rewrite Genv.find_funct_find_funct_ptr in H. auto.
+  rewrite H2. eapply functions_translated; eauto.
+  (* symbol *)
+  rewrite symbols_preserved. destruct (Genv.find_symbol ge id); try discriminate.
+  eapply funct_ptr_translated; eauto.
+Qed.
+
+(** ** Relating stacks *)
+
+Inductive match_stacks (s s':list stackframe) (F: meminj) (m m': mem):
+             list stackframe -> list stackframe -> block -> Prop :=
+  | match_stacks_nil: forall bound1 bound
+        (MG: match_globalenvs F bound1)
+        (BELOW: Ple bound1 bound),
+      match_stacks s s' F m m' nil nil bound
+  | match_stacks_cons: forall res f sp pc rs stk f' sp' rs' stk' bound ctx
+        (MS: match_stacks_inside s s' F m m' stk stk' f' ctx sp' rs')
+        (FB: tr_funbody fenv f'.(fn_stacksize) ctx f f'.(fn_code))
+        (AG: agree_regs F ctx rs rs')
+        (SP: F sp = Some(sp', ctx.(dstk)))
+        (PRIV: range_private F m m' sp' (ctx.(dstk) + ctx.(mstk)) f'.(fn_stacksize))
+        (SSZ1: 0 <= f'.(fn_stacksize) < Int.max_unsigned)
+        (SSZ2: forall ofs, Mem.perm m' sp' ofs Max Nonempty -> 0 <= ofs <= f'.(fn_stacksize))
+        (RES: Ple res ctx.(mreg))
+        (BELOW: Plt sp' bound),
+      match_stacks s s' F m m'
+                   (Stackframe res f (Vptr sp Int.zero) pc rs :: stk)
+                   (Stackframe (sreg ctx res) f' (Vptr sp' Int.zero) (spc ctx pc) rs' :: stk')
+                   bound
+  | match_stacks_untailcall: forall stk res f' sp' rpc rs' stk' bound ctx
+        (MS: match_stacks_inside s s' F m m' stk stk' f' ctx sp' rs')
+        (PRIV: range_private F m m' sp' ctx.(dstk) f'.(fn_stacksize))
+        (SSZ1: 0 <= f'.(fn_stacksize) < Int.max_unsigned)
+        (SSZ2: forall ofs, Mem.perm m' sp' ofs Max Nonempty -> 0 <= ofs <= f'.(fn_stacksize))
+        (RET: ctx.(retinfo) = Some (rpc, res))
+        (BELOW: Plt sp' bound),
+      match_stacks s s' F m m'
+                   stk
+                   (Stackframe res f' (Vptr sp' Int.zero) rpc rs' :: stk')
+                   bound
+
+with match_stacks_inside (s s':list stackframe) (F: meminj) (m m': mem):
+        list stackframe -> list stackframe -> function -> context -> block -> regset -> Prop :=
+  (* | match_stacks_inside_base: forall stk stk' f' ctx sp' rs' *)
+  (*       (MS: match_stacks F m m' stk stk' sp') *)
+  (*       (RET: ctx.(retinfo) = None) *)
+  (*       (DSTK: ctx.(dstk) = 0), *)
+  (*     match_stacks_inside F m m' stk stk' f' ctx sp' rs' *)
+  | match_stacks_inside_inlined: forall res f sp pc rs stk stk' f' ctx sp' rs' ctx'
+        (MS: match_stacks_inside s s' F m m' stk stk' f' ctx' sp' rs')
+        (FB: tr_funbody fenv f'.(fn_stacksize) ctx' f f'.(fn_code))
+        (AG: agree_regs F ctx' rs rs')
+        (SP: F sp = Some(sp', ctx'.(dstk)))
+        (PAD: range_private F m m' sp' (ctx'.(dstk) + ctx'.(mstk)) ctx.(dstk))
+        (RES: Ple res ctx'.(mreg))
+        (RET: ctx.(retinfo) = Some (spc ctx' pc, sreg ctx' res))
+        (BELOW: context_below ctx' ctx)
+        (SBELOW: context_stack_call ctx' ctx),
+      match_stacks_inside s s' F m m'
+                          (Stackframe res f (Vptr sp Int.zero) pc rs :: stk)
+                          stk'
+                          f' ctx sp' rs'.
+
+(** Properties of match_stacks *)
+
+Section MATCH_STACKS.
+
+Variable s s': list stackframe.
+Variable F: meminj.
+Variables m m': mem.
+
+Lemma match_stacks_globalenvs:
+  forall stk stk' bound,
+  match_stacks s s' F m m' stk stk' bound -> exists b, match_globalenvs F b
+with match_stacks_inside_globalenvs:
+  forall stk stk' f ctx sp rs', 
+  match_stacks_inside s s' F m m' stk stk' f ctx sp rs' -> exists b, match_globalenvs F b.
+Proof.
+  induction 1; eauto.
+  induction 1; eauto.
+Qed.
+
+Lemma match_globalenvs_preserves_globals:
+  forall b, match_globalenvs F b -> meminj_preserves_globals ge F.
+Proof.
+  intros. inv H. red. split. eauto. split. eauto.
+  intros. symmetry. eapply IMAGE; eauto.
+Qed. 
+
+Lemma match_stacks_inside_globals:
+  forall stk stk' f ctx sp rs', 
+  match_stacks_inside s s' F m m' stk stk' f ctx sp rs' -> meminj_preserves_globals ge F.
+Proof.
+  intros. exploit match_stacks_inside_globalenvs; eauto. intros [b A]. 
+  eapply match_globalenvs_preserves_globals; eauto.
+Qed.
+
+Lemma match_stacks_bound:
+  forall stk stk' bound bound1,
+  match_stacks s s' F m m' stk stk' bound ->
+  Ple bound bound1 ->
+  match_stacks s s' F m m' stk stk' bound1.
+Proof.
+  intros. inv H.
+  apply match_stacks_nil with bound0. auto. eapply Ple_trans; eauto. 
+  eapply match_stacks_cons; eauto. eapply Plt_le_trans; eauto. 
+  eapply match_stacks_untailcall; eauto. eapply Plt_le_trans; eauto. 
+Qed. 
+
+Variable F1: meminj.
+Variables m1 m1': mem.
+Hypothesis INCR: inject_incr F F1.
+
+Lemma match_stacks_invariant:
+  forall stk stk' bound, match_stacks s s' F m m' stk stk' bound ->
+  forall (INJ: forall b1 b2 delta, 
+               F1 b1 = Some(b2, delta) -> Plt b2 bound -> F b1 = Some(b2, delta))
+         (PERM1: forall b1 b2 delta ofs,
+               F1 b1 = Some(b2, delta) -> Plt b2 bound ->
+               Mem.perm m1 b1 ofs Max Nonempty -> Mem.perm m b1 ofs Max Nonempty)
+         (PERM2: forall b ofs, Plt b bound ->
+               Mem.perm m' b ofs Cur Freeable -> Mem.perm m1' b ofs Cur Freeable)
+         (PERM3: forall b ofs k p, Plt b bound ->
+               Mem.perm m1' b ofs k p -> Mem.perm m' b ofs k p),
+  match_stacks s s' F1 m1 m1' stk stk' bound
+
+with match_stacks_inside_invariant:
+  forall stk stk' f' ctx sp' rs1, 
+  match_stacks_inside s s' F m m' stk stk' f' ctx sp' rs1 ->
+  forall rs2
+         (RS: forall r, Plt r ctx.(dreg) -> rs2#r = rs1#r)
+         (INJ: forall b1 b2 delta, 
+               F1 b1 = Some(b2, delta) -> Ple b2 sp' -> F b1 = Some(b2, delta))
+         (PERM1: forall b1 b2 delta ofs,
+               F1 b1 = Some(b2, delta) -> Ple b2 sp' ->
+               Mem.perm m1 b1 ofs Max Nonempty -> Mem.perm m b1 ofs Max Nonempty)
+         (PERM2: forall b ofs, Ple b sp' ->
+               Mem.perm m' b ofs Cur Freeable -> Mem.perm m1' b ofs Cur Freeable)
+         (PERM3: forall b ofs k p, Ple b sp' ->
+               Mem.perm m1' b ofs k p -> Mem.perm m' b ofs k p),
+  match_stacks_inside s s' F1 m1 m1' stk stk' f' ctx sp' rs2.
+
+Proof.
+  induction 1; intros.
+  (* nil *)
+  apply match_stacks_nil with (bound1 := bound1).
+  inv MG. constructor; auto. 
+  intros. apply IMAGE with delta. eapply INJ; eauto. eapply Plt_le_trans; eauto.
+  auto. auto.
+  (* cons *)
+  apply match_stacks_cons with (ctx := ctx); auto.
+  eapply match_stacks_inside_invariant; eauto.
+  intros; eapply INJ; eauto; xomega. 
+  intros; eapply PERM1; eauto; xomega.
+  intros; eapply PERM2; eauto; xomega.
+  intros; eapply PERM3; eauto; xomega.
+  eapply agree_regs_incr; eauto.
+  eapply range_private_invariant; eauto. 
+  (* untailcall *)
+  apply match_stacks_untailcall with (ctx := ctx); auto. 
+  eapply match_stacks_inside_invariant; eauto.
+  intros; eapply INJ; eauto; xomega.
+  intros; eapply PERM1; eauto; xomega.
+  intros; eapply PERM2; eauto; xomega.
+  intros; eapply PERM3; eauto; xomega.
+  eapply range_private_invariant; eauto. 
+
+  induction 1; intros.
+  (* (* base *) *)
+  (* eapply match_stacks_inside_base; eauto. *)
+  (* eapply match_stacks_invariant; eauto.  *)
+  (* intros; eapply INJ; eauto; xomega. *)
+  (* intros; eapply PERM1; eauto; xomega. *)
+  (* intros; eapply PERM2; eauto; xomega. *)
+  (* intros; eapply PERM3; eauto; xomega. *)
+  (* inlined *)
+  apply match_stacks_inside_inlined with (ctx' := ctx'); auto. 
+  apply IHmatch_stacks_inside; auto.
+  intros. apply RS. red in BELOW. xomega. 
+  apply agree_regs_incr with F; auto. 
+  apply agree_regs_invariant with rs'; auto. 
+  intros. apply RS. red in BELOW. xomega. 
+  eapply range_private_invariant; eauto.
+    intros. split. eapply INJ; eauto. xomega. eapply PERM1; eauto. xomega.
+    intros. eapply PERM2; eauto. xomega.
+Qed.
+
+(* Lemma match_stacks_empty: *)
+(*   forall stk stk' bound, *)
+(*   match_stacks F m m' stk stk' bound -> stk = nil -> stk' = nil *)
+(* with match_stacks_inside_empty: *)
+(*   forall stk stk' f ctx sp rs, *)
+(*   match_stacks_inside F m m' stk stk' f ctx sp rs -> stk = nil -> stk' = nil /\ ctx.(retinfo) = None. *)
+(* Proof. *)
+(*   induction 1; intros. *)
+(*   auto. *)
+(*   discriminate. *)
+(*   exploit match_stacks_inside_empty; eauto. intros [A B]. congruence. *)
+(*   induction 1; intros. *)
+(*   split. eapply match_stacks_empty; eauto. auto. *)
+(*   discriminate. *)
+(* Qed. *)
+
+End MATCH_STACKS.
+
+(** Preservation by assignment to a register *)
+
+Lemma match_stacks_inside_set_reg:
+  forall s s' F m m' stk stk' f' ctx sp' rs' r v, 
+  match_stacks_inside s s' F m m' stk stk' f' ctx sp' rs' ->
+  match_stacks_inside s s' F m m' stk stk' f' ctx sp' (rs'#(sreg ctx r) <- v).
+Proof.
+  intros. eapply match_stacks_inside_invariant; eauto. 
+  intros. apply Regmap.gso. zify. unfold sreg; rewrite shiftpos_eq. xomega.
+Qed.
+
+(** Preservation by a memory store *)
+
+Lemma match_stacks_inside_store:
+  forall s s' F m m' stk stk' f' ctx sp' rs' chunk b ofs v m1 chunk' b' ofs' v' m1', 
+  match_stacks_inside s s' F m m' stk stk' f' ctx sp' rs' ->
+  Mem.store chunk m b ofs v = Some m1 ->
+  Mem.store chunk' m' b' ofs' v' = Some m1' ->
+  match_stacks_inside s s' F m1 m1' stk stk' f' ctx sp' rs'.
+Proof.
+  intros. 
+  eapply match_stacks_inside_invariant; eauto with mem.
+Qed.
+
+(** Preservation by an allocation *)
+
+Lemma match_stacks_inside_alloc_left:
+  forall s s' F m m' stk stk' f' ctx sp' rs',
+  match_stacks_inside s s' F m m' stk stk' f' ctx sp' rs' ->
+  forall sz m1 b F1 delta,
+  Mem.alloc m 0 sz = (m1, b) ->
+  inject_incr F F1 ->
+  F1 b = Some(sp', delta) ->
+  (forall b1, b1 <> b -> F1 b1 = F b1) ->
+  delta >= ctx.(dstk) ->
+  match_stacks_inside s s' F1 m1 m' stk stk' f' ctx sp' rs'.
+Proof.
+  induction 1; intros.
+  (* (* base *) *)
+  (* eapply match_stacks_inside_base; eauto.  *)
+  (* eapply match_stacks_invariant; eauto. *)
+  (* intros. destruct (eq_block b1 b). *)
+  (* subst b1. rewrite H1 in H4; inv H4. eelim Plt_strict; eauto.  *)
+  (* rewrite H2 in H4; auto.  *)
+  (* intros. exploit Mem.perm_alloc_inv; eauto. destruct (eq_block b1 b); intros; auto. *)
+  (* subst b1. rewrite H1 in H4. inv H4. eelim Plt_strict; eauto.  *)
+  (* inlined *)
+  eapply match_stacks_inside_inlined; eauto. 
+  eapply IHmatch_stacks_inside; eauto. destruct SBELOW. omega. 
+  eapply agree_regs_incr; eauto.
+  eapply range_private_invariant; eauto. 
+  intros. exploit Mem.perm_alloc_inv; eauto. destruct (eq_block b0 b); intros.
+  subst b0. rewrite H2 in H5; inv H5. elimtype False; xomega. 
+  rewrite H3 in H5; auto. 
+Qed.
+
+(** Preservation by freeing *)
+
+Lemma match_stacks_free_left:
+  forall s s' F m m' stk stk' sp b lo hi m1,
+  match_stacks s s' F m m' stk stk' sp ->
+  Mem.free m b lo hi = Some m1 ->
+  match_stacks s s' F m1 m' stk stk' sp.
+Proof.
+  intros. eapply match_stacks_invariant; eauto.
+  intros. eapply Mem.perm_free_3; eauto. 
+Qed.
+
+Lemma match_stacks_free_right:
+  forall s s' F m m' stk stk' sp lo hi m1',
+  match_stacks s s' F m m' stk stk' sp ->
+  Mem.free m' sp lo hi = Some m1' ->
+  match_stacks s s' F m m1' stk stk' sp.
+Proof.
+  intros. eapply match_stacks_invariant; eauto. 
+  intros. eapply Mem.perm_free_1; eauto. 
+  intros. eapply Mem.perm_free_3; eauto.
+Qed.
+
+Lemma min_alignment_sound:
+  forall sz n, (min_alignment sz | n) -> Mem.inj_offset_aligned n sz.
+Proof.
+  intros; red; intros. unfold min_alignment in H. 
+  assert (2 <= sz -> (2 | n)). intros.
+    destruct (zle sz 1). omegaContradiction.
+    destruct (zle sz 2). auto. 
+    destruct (zle sz 4). apply Zdivides_trans with 4; auto. exists 2; auto.
+    apply Zdivides_trans with 8; auto. exists 4; auto.
+  assert (4 <= sz -> (4 | n)). intros.
+    destruct (zle sz 1). omegaContradiction.
+    destruct (zle sz 2). omegaContradiction.
+    destruct (zle sz 4). auto.
+    apply Zdivides_trans with 8; auto. exists 2; auto.
+  assert (8 <= sz -> (8 | n)). intros.
+    destruct (zle sz 1). omegaContradiction.
+    destruct (zle sz 2). omegaContradiction.
+    destruct (zle sz 4). omegaContradiction.
+    auto.
+  destruct chunk; simpl in *; auto.
+  apply Zone_divide.
+  apply Zone_divide.
+  apply H2; omega.
+  apply H2; omega.
+Qed.
+
+(** Preservation by external calls *)
+
+Section EXTCALL.
+
+Variables F1 F2: meminj.
+Variables m1 m2 m1' m2': mem.
+Hypothesis MAXPERM: forall b ofs p, Mem.valid_block m1 b -> Mem.perm m2 b ofs Max p -> Mem.perm m1 b ofs Max p.
+Hypothesis MAXPERM': forall b ofs p, Mem.valid_block m1' b -> Mem.perm m2' b ofs Max p -> Mem.perm m1' b ofs Max p.
+Hypothesis UNCHANGED: Mem.unchanged_on (loc_out_of_reach F1 m1) m1' m2'.
+Hypothesis INJ: Mem.inject F1 m1 m1'.
+Hypothesis INCR: inject_incr F1 F2.
+Hypothesis SEP: inject_separated F1 F2 m1 m1'.
+
+Lemma match_stacks_extcall:
+  forall s s' stk stk' bound, 
+  match_stacks s s' F1 m1 m1' stk stk' bound ->
+  Ple bound (Mem.nextblock m1') ->
+  match_stacks s s' F2 m2 m2' stk stk' bound
+with match_stacks_inside_extcall:
+  forall s s' stk stk' f' ctx sp' rs',
+  match_stacks_inside s s' F1 m1 m1' stk stk' f' ctx sp' rs' ->
+  Plt sp' (Mem.nextblock m1') ->
+  match_stacks_inside s s' F2 m2 m2' stk stk' f' ctx sp' rs'.
+Proof.
+  induction 1; intros.
+  apply match_stacks_nil with bound1; auto. 
+    inv MG. constructor; intros; eauto. 
+    destruct (F1 b1) as [[b2' delta']|] eqn:?.
+    exploit INCR; eauto. intros EQ; rewrite H0 in EQ; inv EQ. eapply IMAGE; eauto. 
+    exploit SEP; eauto. intros [A B]. elim B. red. xomega. 
+  eapply match_stacks_cons; eauto. 
+    eapply match_stacks_inside_extcall; eauto. xomega. 
+    eapply agree_regs_incr; eauto. 
+    eapply range_private_extcall; eauto. red; xomega. 
+    intros. apply SSZ2; auto. apply MAXPERM'; auto. red; xomega.
+  eapply match_stacks_untailcall; eauto. 
+    eapply match_stacks_inside_extcall; eauto. xomega. 
+    eapply range_private_extcall; eauto. red; xomega. 
+    intros. apply SSZ2; auto. apply MAXPERM'; auto. red; xomega.
+  induction 1; intros.
+  (* eapply match_stacks_inside_base; eauto. *)
+  (*   eapply match_stacks_extcall; eauto. xomega.  *)
+  eapply match_stacks_inside_inlined; eauto. 
+    eapply agree_regs_incr; eauto. 
+    eapply range_private_extcall; eauto.
+Qed.
+
+End EXTCALL.
+
+(** Change of context corresponding to an inlined tailcall *)
+
+Lemma align_unchanged:
+  forall n amount, amount > 0 -> (amount | n) -> align n amount = n.
+Proof.
+  intros. destruct H0 as [p EQ]. subst n. unfold align. decEq. 
+  apply Zdiv_unique with (b := amount - 1). omega. omega.
+Qed.
+
+Lemma match_stacks_inside_inlined_tailcall:
+  forall s s' F m m' stk stk' f' ctx sp' rs' ctx' f,
+  match_stacks_inside s s' F m m' stk stk' f' ctx sp' rs' ->
+  context_below ctx ctx' ->
+  context_stack_tailcall ctx f ctx' ->
+  ctx'.(retinfo) = ctx.(retinfo) ->
+  range_private F m m' sp' ctx.(dstk) f'.(fn_stacksize) ->
+  tr_funbody fenv f'.(fn_stacksize) ctx' f f'.(fn_code) ->
+  match_stacks_inside s s' F m m' stk stk' f' ctx' sp' rs'.
+Proof.
+  intros. inv H.
+  (* (* base *) *)
+  (* eapply match_stacks_inside_base; eauto. congruence.  *)
+  (* rewrite H1. rewrite DSTK. apply align_unchanged. apply min_alignment_pos. apply Zdivide_0. *)
+  (* inlined *)
+  assert (dstk ctx <= dstk ctx'). rewrite H1. apply align_le. apply min_alignment_pos.
+  eapply match_stacks_inside_inlined; eauto. 
+  red; intros. destruct (zlt ofs (dstk ctx)). apply PAD; omega. apply H3. inv H4. xomega. 
+  congruence. 
+  unfold context_below in *. xomega.
+  unfold context_stack_call in *. omega. 
+Qed.
+
+(** ** Relating states *)
+
+Inductive match_states: list stackframe -> list stackframe -> state -> state -> Prop :=
+  | match_regular_states: forall s s' stk f sp pc rs m stk' f' sp' rs' m' F ctx
+        (MS: match_stacks_inside s s' F m m' stk stk' f' ctx sp' rs')
+        (FB: tr_funbody fenv f'.(fn_stacksize) ctx f f'.(fn_code))
+        (AG: agree_regs F ctx rs rs')
+        (SP: F sp = Some(sp', ctx.(dstk)))
+        (MINJ: Mem.inject F m m')
+        (VB: Mem.valid_block m' sp')
+        (PRIV: range_private F m m' sp' (ctx.(dstk) + ctx.(mstk)) f'.(fn_stacksize))
+        (SSZ1: 0 <= f'.(fn_stacksize) < Int.max_unsigned)
+        (SSZ2: forall ofs, Mem.perm m' sp' ofs Max Nonempty -> 0 <= ofs <= f'.(fn_stacksize)),
+      match_states s s'
+                   (State stk f (Vptr sp Int.zero) pc rs m)
+                   (State stk' f' (Vptr sp' Int.zero) (spc ctx pc) rs' m')
+  | match_call_regular_states: forall s s' stk f vargs m stk' f' sp' rs' m' F ctx ctx' pc' pc1' rargs
+        (MS: match_stacks_inside s s' F m m' stk stk' f' ctx sp' rs')
+        (FB: tr_funbody fenv f'.(fn_stacksize) ctx f f'.(fn_code))
+        (BELOW: context_below ctx' ctx)
+        (NOP: f'.(fn_code)!pc' = Some(Inop pc1'))
+        (MOVES: tr_moves f'.(fn_code) pc1' (sregs ctx' rargs) (sregs ctx f.(fn_params)) (spc ctx f.(fn_entrypoint)))
+        (VINJ: list_forall2 (val_reg_charact F ctx' rs') vargs rargs)
+        (MINJ: Mem.inject F m m')
+        (VB: Mem.valid_block m' sp')
+        (PRIV: range_private F m m' sp' ctx.(dstk) f'.(fn_stacksize))
+        (SSZ1: 0 <= f'.(fn_stacksize) < Int.max_unsigned)
+        (SSZ2: forall ofs, Mem.perm m' sp' ofs Max Nonempty -> 0 <= ofs <= f'.(fn_stacksize)),
+      match_states s s'
+                   (Callstate stk (Internal f) vargs m)
+                   (State stk' f' (Vptr sp' Int.zero) pc' rs' m')
+  | match_return_states: forall s s' stk v m stk' v' m' F
+        (MS: match_stacks s s' F m m' stk stk' (Mem.nextblock m'))
+        (VINJ: val_inject F v v')
+        (MINJ: Mem.inject F m m'),
+      match_states s s'
+                   (Returnstate stk v m)
+                   (Returnstate stk' v' m')
+  | match_return_regular_states: forall s s' stk v m stk' f' sp' rs' m' F ctx pc' or rinfo
+        (MS: match_stacks_inside s s' F m m' stk stk' f' ctx sp' rs')
+        (RET: ctx.(retinfo) = Some rinfo)
+        (AT: f'.(fn_code)!pc' = Some(inline_return ctx or rinfo))
+        (VINJ: match or with None => v = Vundef | Some r => val_inject F v rs'#(sreg ctx r) end)
+        (MINJ: Mem.inject F m m')
+        (VB: Mem.valid_block m' sp')
+        (PRIV: range_private F m m' sp' ctx.(dstk) f'.(fn_stacksize))
+        (SSZ1: 0 <= f'.(fn_stacksize) < Int.max_unsigned)
+        (SSZ2: forall ofs, Mem.perm m' sp' ofs Max Nonempty -> 0 <= ofs <= f'.(fn_stacksize)),
+      match_states s s'
+                   (Returnstate stk v m)
+                   (State stk' f' (Vptr sp' Int.zero) pc' rs' m').
+
+Inductive match_call: list stackframe -> list stackframe -> state -> state -> Prop :=
+  | match_call_states: forall s s' stk fd args m stk' fd' args' m' F
+        (MS: match_stacks s s' F m m' stk stk' (Mem.nextblock m'))
+        (FD: fundef_weak_sim
+               (common_fundef_dec (F:=function)) fn_sig
+               (common_fundef_dec (F:=function)) fn_sig
+               ge tge fd fd')
+        (VINJ: val_list_inject F args args')
+        (MINJ: Mem.inject F m m'),
+      match_call s s'
+                 (Callstate stk fd args m)
+                 (Callstate stk' fd' args' m')
+.
+
+(** ** Forward simulation *)
+
+Definition measure (S: state) : nat :=
+  match S with
+  | State _ _ _ _ _ _ => 1%nat
+  | Callstate _ _ _ _ => 0%nat
+  | Returnstate _ _ _ => 0%nat
+  end.
+
+Lemma tr_funbody_inv:
+  forall sz cts f c pc i,
+  tr_funbody fenv sz cts f c -> f.(fn_code)!pc = Some i -> tr_instr fenv sz cts pc i c.
+Proof.
+  intros. inv H. eauto. 
+Qed.
+
+Theorem step_simulation:
+  forall s s' S1 t S2,
+  step ge S1 t S2 ->
+  forall S1' (MS: match_states s s' S1 S1'),
+  (exists S2', plus step tge S1' t S2' /\ (match_states s s' S2 S2' \/ match_call s s' S2 S2'))
+  \/ (measure S2 < measure S1 /\ t = E0 /\ (match_states s s' S2 S1' \/ match_call s s' S2 S1'))%nat.
+Proof.
+  induction 1; intros; inv MS.
+
+(* nop *)
+  exploit tr_funbody_inv; eauto. intros TR; inv TR.
+  left; econstructor; split. 
+  eapply plus_one. eapply exec_Inop; eauto.
+  left. econstructor; eauto.
+
+(* op *)
+  exploit tr_funbody_inv; eauto. intros TR; inv TR.
+  exploit eval_operation_inject. 
+    eapply match_stacks_inside_globals; eauto.
+    eexact SP.
+    instantiate (2 := rs##args). instantiate (1 := rs'##(sregs ctx args)). eapply agree_val_regs; eauto.
+    eexact MINJ. eauto.
+  fold (sop ctx op). intros [v' [A B]].
+  left; econstructor; split.
+  eapply plus_one. eapply exec_Iop; eauto. erewrite eval_operation_preserved; eauto.
+  exact symbols_preserved. 
+  left. econstructor; eauto.
+  apply match_stacks_inside_set_reg; eauto.
+  apply agree_set_reg; auto. 
+  
+(* load *)
+  exploit tr_funbody_inv; eauto. intros TR; inv TR.
+  exploit eval_addressing_inject. 
+    eapply match_stacks_inside_globals; eauto.
+    eexact SP.
+    instantiate (2 := rs##args). instantiate (1 := rs'##(sregs ctx args)). eapply agree_val_regs; eauto.
+    eauto.
+  fold (saddr ctx addr). intros [a' [P Q]].
+  exploit Mem.loadv_inject; eauto. intros [v' [U V]].
+  assert (eval_addressing tge (Vptr sp' Int.zero) (saddr ctx addr) rs' ## (sregs ctx args) = Some a').
+  rewrite <- P. apply eval_addressing_preserved. exact symbols_preserved.
+  left; econstructor; split.
+  eapply plus_one. eapply exec_Iload; eauto.
+  left. econstructor; eauto. 
+  apply match_stacks_inside_set_reg; eauto.
+  apply agree_set_reg; auto. 
+
+(* store *)
+  exploit tr_funbody_inv; eauto. intros TR; inv TR.
+  exploit eval_addressing_inject. 
+    eapply match_stacks_inside_globals; eauto.
+    eexact SP.
+    instantiate (2 := rs##args). instantiate (1 := rs'##(sregs ctx args)). eapply agree_val_regs; eauto.
+    eauto.
+  fold saddr. intros [a' [P Q]].
+  exploit Mem.storev_mapped_inject; eauto. eapply agree_val_reg; eauto. 
+  intros [m1' [U V]].
+  assert (eval_addressing tge (Vptr sp' Int.zero) (saddr ctx addr) rs' ## (sregs ctx args) = Some a').
+    rewrite <- P. apply eval_addressing_preserved. exact symbols_preserved.
+  left; econstructor; split.
+  eapply plus_one. eapply exec_Istore; eauto.
+  destruct a; simpl in H1; try discriminate.
+  destruct a'; simpl in U; try discriminate.
+  left. econstructor; eauto.
+  eapply match_stacks_inside_store; eauto.
+  eapply Mem.store_valid_block_1; eauto.
+  eapply range_private_invariant; eauto.
+  intros; split; auto. eapply Mem.perm_store_2; eauto.
+  intros; eapply Mem.perm_store_1; eauto.
+  intros. eapply SSZ2. eapply Mem.perm_store_2; eauto.
+
+(* call *)
+  exploit match_stacks_inside_globalenvs; eauto. intros [bound G].
+  exploit find_function_agree; eauto. intros [fd' [A B]].
+  exploit tr_funbody_inv; eauto. intros TR; inv TR.
+(* not inlined *)
+  left; econstructor; split.
+  eapply plus_one. eapply exec_Icall; eauto.
+  eapply sig_preserved; eauto.
+  right. econstructor; eauto.
+  eapply match_stacks_cons; eauto. 
+  eapply agree_val_regs; eauto. 
+(* inlined *)
+  assert (fd = Internal f0).
+    simpl in H0. destruct (Genv.find_symbol ge id) as [b|] eqn:?; try discriminate.
+    exploit (funenv_program_compat prog); eauto. instantiate (1 := b). admit. intros. 
+    unfold ge in H0. admit. (* congruence. *) (* easy *)
+  subst fd.
+  right; split. simpl; omega. split. auto. 
+  left. econstructor; eauto. 
+  eapply match_stacks_inside_inlined; eauto.
+  red; intros. apply PRIV. inv H13. destruct H16. xomega.
+  apply agree_val_regs_gen; auto.
+  red; intros; apply PRIV. destruct H16. omega. 
+
+(* tailcall *)
+  exploit match_stacks_inside_globalenvs; eauto. intros [bound G].
+  exploit find_function_agree; eauto. intros [fd' [A B]].
+  assert (PRIV': range_private F m' m'0 sp' (dstk ctx) f'.(fn_stacksize)).
+    eapply range_private_free_left; eauto. inv FB. rewrite <- H4. auto. 
+  exploit tr_funbody_inv; eauto. intros TR; inv TR.
+(* within the original function *)
+  inv MS0; try congruence.
+  (* assert (X: { m1' | Mem.free m'0 sp' 0 (fn_stacksize f') = Some m1'}). *)
+  (*   apply Mem.range_perm_free. red; intros. *)
+  (*   destruct (zlt ofs f.(fn_stacksize)).  *)
+  (*   replace ofs with (ofs + dstk ctx) by omega. eapply Mem.perm_inject; eauto. *)
+  (*   eapply Mem.free_range_perm; eauto. omega. *)
+  (*   inv FB. eapply range_private_perms; eauto. xomega. *)
+  (* destruct X as [m1' FREE]. *)
+  (* left; econstructor; split. *)
+  (* eapply plus_one. eapply exec_Itailcall; eauto. *)
+  (* eapply sig_preserved; eauto. *)
+  (* econstructor; eauto. *)
+  (* eapply match_stacks_bound with (bound := sp').  *)
+  (* eapply match_stacks_invariant; eauto. *)
+  (*   intros. eapply Mem.perm_free_3; eauto.  *)
+  (*   intros. eapply Mem.perm_free_1; eauto.  *)
+  (*   intros. eapply Mem.perm_free_3; eauto. *)
+  (* erewrite Mem.nextblock_free; eauto. red in VB; xomega. *)
+  (* eapply agree_val_regs; eauto. *)
+  (* eapply Mem.free_right_inject; eauto. eapply Mem.free_left_inject; eauto. *)
+  (* (* show that no valid location points into the stack block being freed *) *)
+  (* intros. rewrite DSTK in PRIV'. exploit (PRIV' (ofs + delta)). omega. intros [P Q].  *)
+  (* eelim Q; eauto. replace (ofs + delta - delta) with ofs by omega.  *)
+  (* apply Mem.perm_max with k. apply Mem.perm_implies with p; auto with mem. *)
+(* turned into a call *)
+  left; econstructor; split.
+  eapply plus_one. eapply exec_Icall; eauto.
+  eapply sig_preserved; eauto.
+  right. econstructor; eauto.
+  eapply match_stacks_untailcall; eauto.
+  eapply match_stacks_inside_invariant; eauto. 
+    intros. eapply Mem.perm_free_3; eauto.
+  eapply agree_val_regs; eauto.
+  eapply Mem.free_left_inject; eauto.
+(* inlined *)
+  assert (fd = Internal f0).
+    simpl in H0. destruct (Genv.find_symbol ge id) as [b|] eqn:?; try discriminate.
+    exploit (funenv_program_compat prog); eauto. instantiate (1 := b). admit. intros. 
+    unfold ge in H0. admit. (* congruence. *) (* easy *)
+  subst fd.
+  right; split. simpl; omega. split. auto. 
+  left. econstructor; eauto.
+  eapply match_stacks_inside_inlined_tailcall; eauto.
+  eapply match_stacks_inside_invariant; eauto.
+    intros. eapply Mem.perm_free_3; eauto.
+  apply agree_val_regs_gen; auto.
+  eapply Mem.free_left_inject; eauto.
+  red; intros; apply PRIV'. 
+    assert (dstk ctx <= dstk ctx'). red in H14; rewrite H14. apply align_le. apply min_alignment_pos.
+    omega.
+
+(* builtin *)
+  exploit tr_funbody_inv; eauto. intros TR; inv TR.
+  exploit external_call_mem_inject; eauto. 
+    eapply match_stacks_inside_globals; eauto.
+    instantiate (1 := rs'##(sregs ctx args)). eapply agree_val_regs; eauto. 
+  intros [F1 [v1 [m1' [A [B [C [D [E [J K]]]]]]]]].
+  left; econstructor; split.
+  eapply plus_one. eapply exec_Ibuiltin; eauto. 
+    eapply external_call_symbols_preserved; eauto. 
+    exact symbols_preserved. exact varinfo_preserved.
+  left. econstructor.
+    eapply match_stacks_inside_set_reg. 
+    eapply match_stacks_inside_extcall with (F1 := F) (F2 := F1) (m1 := m) (m1' := m'0); eauto.
+    intros; eapply external_call_max_perm; eauto. 
+    intros; eapply external_call_max_perm; eauto. 
+  auto. 
+  eapply agree_set_reg. eapply agree_regs_incr; eauto. auto. auto. 
+  apply J; auto.
+  auto. 
+  eapply external_call_valid_block; eauto. 
+  eapply range_private_extcall; eauto. 
+    intros; eapply external_call_max_perm; eauto. 
+  auto. 
+  intros. apply SSZ2. eapply external_call_max_perm; eauto. 
+
+(* cond *)
+  exploit tr_funbody_inv; eauto. intros TR; inv TR.
+  assert (eval_condition cond rs'##(sregs ctx args) m' = Some b).
+    eapply eval_condition_inject; eauto. eapply agree_val_regs; eauto. 
+  left; econstructor; split.
+  eapply plus_one. eapply exec_Icond; eauto. 
+  destruct b; left; econstructor; eauto. 
+
+(* jumptable *)
+  exploit tr_funbody_inv; eauto. intros TR; inv TR.
+  assert (val_inject F rs#arg rs'#(sreg ctx arg)). eapply agree_val_reg; eauto.
+  rewrite H0 in H2; inv H2. 
+  left; econstructor; split.
+  eapply plus_one. eapply exec_Ijumptable; eauto.
+  rewrite list_nth_z_map. rewrite H1. simpl; reflexivity. 
+  left. econstructor; eauto. 
+
+(* return *)
+  exploit tr_funbody_inv; eauto. intros TR; inv TR.
+  (* not inlined *)
+  inv MS0; try congruence.
+  (* assert (X: { m1' | Mem.free m'0 sp' 0 (fn_stacksize f') = Some m1'}). *)
+  (*   apply Mem.range_perm_free. red; intros. *)
+  (*   destruct (zlt ofs f.(fn_stacksize)). *)
+  (*   replace ofs with (ofs + dstk ctx) by omega. eapply Mem.perm_inject; eauto. *)
+  (*   eapply Mem.free_range_perm; eauto. omega. *)
+  (*   inv FB. eapply range_private_perms; eauto. *)
+  (*   generalize (Zmax_spec (fn_stacksize f) 0). destruct (zlt 0 (fn_stacksize f)); omega. *)
+  (* destruct X as [m1' FREE]. *)
+  (* left; econstructor; split. *)
+  (* eapply plus_one. eapply exec_Ireturn; eauto. *)
+  (* econstructor; eauto. *)
+  (* eapply match_stacks_bound with (bound := sp'). *)
+  (* eapply match_stacks_invariant; eauto. *)
+  (*   intros. eapply Mem.perm_free_3; eauto. *)
+  (*   intros. eapply Mem.perm_free_1; eauto. *)
+  (*   intros. eapply Mem.perm_free_3; eauto. *)
+  (* erewrite Mem.nextblock_free; eauto. red in VB; xomega. *)
+  (* destruct or; simpl. apply agree_val_reg; auto. auto. *)
+  (* eapply Mem.free_right_inject; eauto. eapply Mem.free_left_inject; eauto. *)
+  (* show that no valid location points into the stack block being freed *)
+  (* intros. inversion FB; subst. *)
+  (* assert (PRIV': range_private F m' m'0 sp' (dstk ctx) f'.(fn_stacksize)). *)
+  (*   rewrite H8 in PRIV. eapply range_private_free_left; eauto.  *)
+  (* rewrite DSTK in PRIV'. exploit (PRIV' (ofs + delta)). omega. intros [A B].  *)
+  (* eelim B; eauto. replace (ofs + delta - delta) with ofs by omega.  *)
+  (* apply Mem.perm_max with k. apply Mem.perm_implies with p; auto with mem. *)
+
+  (* inlined *)
+  right. split. simpl. omega. split. auto. 
+  left. econstructor; eauto.
+  eapply match_stacks_inside_invariant; eauto. 
+    intros. eapply Mem.perm_free_3; eauto.
+  destruct or; simpl. apply agree_val_reg; auto. auto.
+  eapply Mem.free_left_inject; eauto.
+  inv FB. rewrite H4 in PRIV. eapply range_private_free_left; eauto. 
+
+(* internal function, not inlined *)
+  (* assert (A: exists f', tr_function fenv f f' /\ fd' = Internal f'). *)
+  (*   Errors.monadInv FD. exists x. split; auto. eapply transf_function_spec; eauto.  *)
+  (* destruct A as [f' [TR EQ]]. inversion TR; subst. *)
+  (* exploit Mem.alloc_parallel_inject. eauto. eauto. apply Zle_refl.  *)
+  (*   instantiate (1 := fn_stacksize f'). inv H0. xomega.  *)
+  (* intros [F' [m1' [sp' [A [B [C [D E]]]]]]]. *)
+  (* left; econstructor; split. *)
+  (* eapply plus_one. eapply exec_function_internal; eauto. *)
+  (* rewrite H5. econstructor. *)
+  (* instantiate (1 := F'). apply match_stacks_inside_base. *)
+  (* assert (SP: sp' = Mem.nextblock m'0) by (eapply Mem.alloc_result; eauto). *)
+  (* rewrite <- SP in MS0.  *)
+  (* eapply match_stacks_invariant; eauto. *)
+  (*   intros. destruct (eq_block b1 stk).  *)
+  (*   subst b1. rewrite D in H7; inv H7. subst b2. eelim Plt_strict; eauto.   *)
+  (*   rewrite E in H7; auto.  *)
+  (*   intros. exploit Mem.perm_alloc_inv. eexact H. eauto.  *)
+  (*   destruct (eq_block b1 stk); intros; auto.  *)
+  (*   subst b1. rewrite D in H7; inv H7. subst b2. eelim Plt_strict; eauto.   *)
+  (*   intros. eapply Mem.perm_alloc_1; eauto.  *)
+  (*   intros. exploit Mem.perm_alloc_inv. eexact A. eauto.  *)
+  (*   rewrite dec_eq_false; auto. *)
+  (* auto. auto. auto.  *)
+  (* rewrite H4. apply agree_regs_init_regs. eauto. auto. inv H0; auto. congruence. auto. *)
+  (* eapply Mem.valid_new_block; eauto. *)
+  (* red; intros. split. *)
+  (* eapply Mem.perm_alloc_2; eauto. inv H0; xomega. *)
+  (* intros; red; intros. exploit Mem.perm_alloc_inv. eexact H. eauto. *)
+  (* destruct (eq_block b stk); intros.  *)
+  (* subst. rewrite D in H8; inv H8. inv H0; xomega. *)
+  (* rewrite E in H8; auto. eelim Mem.fresh_block_alloc. eexact A. eapply Mem.mi_mappedblocks; eauto. *)
+  (* auto. *)
+  (* intros. exploit Mem.perm_alloc_inv; eauto. rewrite dec_eq_true. omega.  *)
+
+(* internal function, inlined *)
+  inversion FB; subst.
+  exploit Mem.alloc_left_mapped_inject. 
+    eauto.
+    eauto.
+    (* sp' is valid *)
+    instantiate (1 := sp'). auto.
+    (* offset is representable *)
+    instantiate (1 := dstk ctx). generalize (Zmax2 (fn_stacksize f) 0). omega.
+    (* size of target block is representable *)
+    intros. right. exploit SSZ2; eauto with mem. inv FB; omega.
+    (* we have full permissions on sp' at and above dstk ctx *)
+    intros. apply Mem.perm_cur. apply Mem.perm_implies with Freeable; auto with mem.
+    eapply range_private_perms; eauto. xomega.
+    (* offset is aligned *)
+    replace (fn_stacksize f - 0) with (fn_stacksize f) by omega.
+    inv FB. apply min_alignment_sound; auto.
+    (* nobody maps to (sp, dstk ctx...) *)
+    intros. exploit (PRIV (ofs + delta')); eauto. xomega.
+    intros [A B]. eelim B; eauto.
+    replace (ofs + delta' - delta') with ofs by omega.
+    apply Mem.perm_max with k. apply Mem.perm_implies with p; auto with mem.
+  intros [F' [A [B [C D]]]].
+  exploit tr_moves_init_regs; eauto. intros [rs'' [P [Q R]]].
+  left; econstructor; split. 
+  eapply plus_left. eapply exec_Inop; eauto. eexact P. traceEq.
+  left. econstructor.
+  eapply match_stacks_inside_alloc_left; eauto.
+  eapply match_stacks_inside_invariant; eauto.
+  omega.
+  auto.
+  apply agree_regs_incr with F; auto.
+  auto. auto. auto.
+  rewrite H2. eapply range_private_alloc_left; eauto.
+  auto. auto.
+
+(* external function *)
+  (* exploit match_stacks_globalenvs; eauto. intros [bound MG]. *)
+  (* exploit external_call_mem_inject; eauto.  *)
+  (*   eapply match_globalenvs_preserves_globals; eauto. *)
+  (* intros [F1 [v1 [m1' [A [B [C [D [E [J K]]]]]]]]]. *)
+  (* simpl in FD. inv FD.  *)
+  (* left; econstructor; split. *)
+  (* eapply plus_one. eapply exec_function_external; eauto.  *)
+  (*   eapply external_call_symbols_preserved; eauto.  *)
+  (*   exact symbols_preserved. exact varinfo_preserved. *)
+  (* econstructor. *)
+  (*   eapply match_stacks_bound with (Mem.nextblock m'0). *)
+  (*   eapply match_stacks_extcall with (F1 := F) (F2 := F1) (m1 := m) (m1' := m'0); eauto. *)
+  (*   intros; eapply external_call_max_perm; eauto.  *)
+  (*   intros; eapply external_call_max_perm; eauto. *)
+  (*   xomega. *)
+  (*   eapply external_call_nextblock; eauto.  *)
+  (*   auto. auto. *)
+
+(* return fron noninlined function *)
+  inv MS0.
+  (* normal case *)
+  left; econstructor; split.
+  eapply plus_one. eapply exec_return.
+  left. econstructor; eauto. 
+  apply match_stacks_inside_set_reg; eauto. 
+  apply agree_set_reg; auto.
+  (* untailcall case *)
+  inv MS; try congruence.
+  rewrite RET in RET0; inv RET0.
+(*
+  assert (rpc = pc). unfold spc in H0; unfold node in *; xomega.
+  assert (res0 = res). unfold sreg in H1; unfold reg in *; xomega.
+  subst rpc res0.
+*)
+  left; econstructor; split.
+  eapply plus_one. eapply exec_return.
+  left. eapply match_regular_states. 
+  eapply match_stacks_inside_set_reg; eauto.
+  auto. 
+  apply agree_set_reg; auto.
+  auto. auto. auto.
+  red; intros. destruct (zlt ofs (dstk ctx)). apply PAD; omega. apply PRIV; omega.
+  auto. auto. 
+  
+(* return from inlined function *)
+  inv MS0; try congruence. rewrite RET0 in RET; inv RET. 
+  unfold inline_return in AT. 
+  assert (PRIV': range_private F m m' sp' (dstk ctx' + mstk ctx') f'.(fn_stacksize)).
+    red; intros. destruct (zlt ofs (dstk ctx)). apply PAD. omega. apply PRIV. omega.
+  destruct or.
+  (* with a result *)
+  left; econstructor; split. 
+  eapply plus_one. eapply exec_Iop; eauto. simpl. reflexivity. 
+  left. econstructor; eauto. apply match_stacks_inside_set_reg; eauto. apply agree_set_reg; auto.
+  (* without a result *)
+  left; econstructor; split. 
+  eapply plus_one. eapply exec_Inop; eauto.
+  left. econstructor; eauto. subst vres. apply agree_set_reg_undef'; auto.
+Qed.
+
+Lemma match_states_state_lsim s s' st:
+  match_states s s' st <1= state_lsim mrelT_ops_extends fprog ftprog s s' tt tt (WF.from_nat (measure st)) st.
+Proof.
+  admit.
+Qed.
+
+Lemma transf_function'_lsim
+      f f' (Hf: Inlining.transf_function fenv f = OK f'):
+  function_lsim mrelT_ops_extends fprog ftprog f f'.
+Proof.
+  constructor. repeat intro. pfold. constructor; subst; auto.
+  { intros ? Hfinal. inv Hfinal. }
+  intros. inversion Hst2_src. subst.
+  exists WF.elt. eexists. exists tt.
+  split; [left; apply plus_one; eauto|].
+  { econstructor; eauto.
+    match goal with
+      | [|- ?b = _] =>
+        instantiate (1 := snd b); instantiate (1 := fst b); auto
+    end.
+  }
+  split; [reflexivity|].
+  admit.
+Qed.
+
+End FUTURE.
+
+Lemma Inlining_program_sim:
+  program_sim
+    (@common_fundef_dec function) fn_sig
+    (@common_fundef_dec function) fn_sig
+    (@Errors.OK _)
+    (function_lsim mrelT_ops_extends)
+    prog tprog.
+Proof.
+  generalize transf_function'_lsim.
+  destruct prog as [defs main]. clear prog. simpl in *.
+  unfold transf_program, transform_partial_program in TRANSF.
+  unfold transform_partial_program2 in TRANSF.
+  admit.
+Qed.
+
+End INLINING.
